$$
s(\xi) = \frac{\xi + 1}{2}(s_{i+1} - s_i)
$$

$$
\frac{\partial{s}}{\partial \xi} = \frac{1}{2}(s_{i+1} - s_i)
$$


$$
\frac{\partial{x}}{\partial \xi} = \frac{\partial{s}}{\partial \xi} \frac{\partial{x}}{\partial s}
$$

$$
\frac{\partial^2 x}{\partial \xi^2} = \frac{\partial}{\partial \xi}\left(\frac{\partial{s}}{\partial \xi} \frac{\partial{x}}{\partial s}  \right)
$$

$$
\frac{\partial^2 x}{\partial \xi^2} = 
\frac{\partial^2 {s}}{\partial \xi^2} \frac{\partial x}{\partial s}
+
\left(\frac{\partial{s}}{\partial \xi} \right)^2 \frac{\partial^2 x}{\partial s^2}
$$

